

2024-03-22

Boolean Formula Simplification Exercise

1. Simplify $wx + wxy + w'yz + w'y'z + w'xyz'$
2. Simplify $x'y'z' + x'y'z + x'yz + xy'z + xyz$
3. Simplify $abc' + ab'c + a'bc + abc$
4. Simplify $x'z + xy'z + xyz$
5. Simplify $x'y'z' + x'yz + xyz$
6. Simplify $x'y'z + w'xz + wxyz' + wxz + w'xyz$
7. Simplify $a'b'c' + a'b'c + abc + ab'c$
8. Simplify $a'b'c' + a'bc' + a'bc + ab'c + abc' + abc$
9. Use only two-input NAND gates to implement $f = w'y' + xyz + wyz' + x'y'z$
10. Use only two-input NAND gates to implement $f = abc + abd + a'c'd + a'b'c$

P1a.	$a + b = b + a$	P1b.	$ab = ba$	Commutative
P2a.	$a + (b + c) = (a + b) + c$	P2b.	$a(bc) = (ab)c$	Associative
P3a.	$a + 0 = a$	P3b.	$a \cdot 1 = a$	Identity
P3aa.	$0 + a = a$	P3bb.	$1 \cdot a = a$	
P4a.	$a + 1 = 1$	P4b.	$a \cdot 0 = 0$	Null
P4aa.	$1 + a = 1$	P4bb.	$0 \cdot a = 0$	
P5a.	$a + a' = 1$	P5b.	$a \cdot a' = 0$	Complement
P5aa.	$a' + a = 1$	P5bb.	$a' \cdot a = 0$	
P6a.	$a + a = a$	P6b.	$a \cdot a = a$	Idempotency
P7.	$(a')' = a$			Involution
P8a.	$a(b + c) = ab + ac$	P8b.	$a + bc = (a + b)(a + c)$	Distributive
P9a.	$ab + ab' = a$	P9b.	$(a + b)(a + b') = a$	Adjacency
P9aa.	$a'b' + a'b + ab + ab' = 1$	P9bb.	$(a' + b')(a' + b)(a + b)(a + b') = 0$	
P10a.	$a + a'b = a + b$	P10b.	$a(a' + b) = ab$	Simplification
P11a.	$(a + b)' = a'b'$	P11b.	$(ab)' = a' + b'$	DeMorgan
P11aa.	$(a + b + c \dots)' = a'b'c' \dots$	P11bb.	$(abc \dots)' = a' + b' + c' \dots$	
P12a.	$a + ab = a$	P12b.	$a(a + b) = a$	Absorption
P13a.	$at_1 + a't_2 + t_1t_2 = at_1 + a't_2$	P13b.	$(a + t_1)(a' + t_2)(t_1 + t_2) = (a + t_1)(a' + t_2)$	Consensus
P14a.	$ab + a'c = (a + c)(a' + b)$			